progress

TestModels/Composite/dafny/DependencyProject/src/Index.dfy
@@ -1,3 +1,30 @@
-module DependencyProject {
+// Copyright Amazon.com Inc. or its affiliates. All Rights Reserved.
+// SPDX-License-Identifier: Apache-2.0
+include "DependencyProjectImpl.dfy"
 
+module {:extern "simple.composite.dependencyproject.internaldafny" } DependencyProject refines AbstractSimpleTypesIntegerService {
+    import Operations = DependencyProjectImpl
+
+    function method DefaultDependencyProjectConfig(): DependencyProjectConfig {
+       DependencyProjectConfig
+    }
+
+    method DependencyProject(config: DependencyProjectConfig)
+    returns (res: Result<ISimpleTypesIntegerClient, Error>) {
+        var client := new DependencyProjectClient(Operations.Config);
+        return Success(client);
+    }
+
+    class DependencyProjectClient... {
+        predicate ValidState()
+        {
+            && Operations.ValidInternalConfig?(config)
+            && Modifies == Operations.ModifiesInternalConfig(config) + {History}
+        }
+        constructor(config: Operations.InternalConfig) {
+            this.config := config;
+            History := new ISimpleTypesIntegerClientCallHistory();
+            Modifies := Operations.ModifiesInternalConfig(config) + {History};
+        }
+    }
 }
