TestModels/Composite/dafny/PrimaryProject/Model/primary-project.smithy
@@ -1,0 +1,27 @@
+namespace simple.composite.primaryproject
+
+use simple.composite.dependencyproject#DependencyService
+use simple.composite.dependencyproject#IdentityOperationInput
+use simple.composite.dependencyproject#IdentityOperationOutput
+
+@aws.polymorph#localService(
+  sdkId: "PrimaryProject",
+  config: PrimaryProjectConfig,
+) service PrimaryProject {
+  version: "2021-11-01",
+  resources: [],
+  operations: [ IdentityOperation, IdentityOperationOnDependency ],
+  errors: [],
+}
+
+structure PrimaryProjectConfig {}
+
+operation IdentityOperation {
+  input: IdentityOperationInput,
+  output: IdentityOperationOutput,
+}
+
+operation IdentityOperationOnDependency {
+  input: IdentityOperationInput,
+  output: IdentityOperationOutput,
+}
